program_logic/hoare.v
@@ -1,35 +1,35 @@
 From program_logic Require Export weakestpre viewshifts.
 
 Definition ht {Λ Σ} (E : coPset) (P : iProp Λ Σ)
-    (e : expr Λ) (Q : val Λ → iProp Λ Σ) : iProp Λ Σ := (□ (P → wp E e Q))%I.
+    (e : expr Λ) (Φ : val Λ → iProp Λ Σ) : iProp Λ Σ := (□ (P → wp E e Φ))%I.
 Instance: Params (@ht) 3.
 
-Notation "{{ P } } e @ E {{ Q } }" := (ht E P e Q)
-  (at level 74, format "{{  P  } }  e  @  E  {{  Q  } }") : uPred_scope.
-Notation "{{ P } } e @ E {{ Q } }" := (True ⊑ ht E P e Q)
-  (at level 74, format "{{  P  } }  e  @  E  {{  Q  } }") : C_scope.
+Notation "{{ P } } e @ E {{ Φ } }" := (ht E P e Φ)
+  (at level 74, format "{{  P  } }  e  @  E  {{  Φ  } }") : uPred_scope.
+Notation "{{ P } } e @ E {{ Φ } }" := (True ⊑ ht E P e Φ)
+  (at level 74, format "{{  P  } }  e  @  E  {{  Φ  } }") : C_scope.
 
 Section hoare.
 Context {Λ : language} {Σ : iFunctor}.
-Implicit Types P : iProp Λ Σ.
-Implicit Types Q : val Λ → iProp Λ Σ.
+Implicit Types P Q : iProp Λ Σ.
+Implicit Types Φ Ψ : val Λ → iProp Λ Σ.
 Implicit Types v : val Λ.
 Import uPred.
 
 Global Instance ht_ne E n :
   Proper (dist n ==> eq==>pointwise_relation _ (dist n) ==> dist n) (@ht Λ Σ E).
-Proof. by intros P P' HP e ? <- Q Q' HQ; rewrite /ht HP; setoid_rewrite HQ. Qed.
+Proof. by intros P P' HP e ? <- Φ Φ' HΦ; rewrite /ht HP; setoid_rewrite HΦ. Qed.
 Global Instance ht_proper E :
   Proper ((≡) ==> eq ==> pointwise_relation _ (≡) ==> (≡)) (@ht Λ Σ E).
-Proof. by intros P P' HP e ? <- Q Q' HQ; rewrite /ht HP; setoid_rewrite HQ. Qed.
-Lemma ht_mono E P P' Q Q' e :
-  P ⊑ P' → (∀ v, Q' v ⊑ Q v) → {{ P' }} e @ E {{ Q' }} ⊑ {{ P }} e @ E {{ Q }}.
+Proof. by intros P P' HP e ? <- Φ Φ' HΦ; rewrite /ht HP; setoid_rewrite HΦ. Qed.
+Lemma ht_mono E P P' Φ Φ' e :
+  P ⊑ P' → (∀ v, Φ' v ⊑ Φ v) → {{ P' }} e @ E {{ Φ' }} ⊑ {{ P }} e @ E {{ Φ }}.
 Proof. by intros; apply always_mono, impl_mono, wp_mono. Qed.
 Global Instance ht_mono' E :
   Proper (flip (⊑) ==> eq ==> pointwise_relation _ (⊑) ==> (⊑)) (@ht Λ Σ E).
-Proof. by intros P P' HP e ? <- Q Q' HQ; apply ht_mono. Qed.
+Proof. by intros P P' HP e ? <- Φ Φ' HΦ; apply ht_mono. Qed.
 
-Lemma ht_alt E P Q e : (P ⊑ wp E e Q) → {{ P }} e @ E {{ Q }}.
+Lemma ht_alt E P Φ e : (P ⊑ wp E e Φ) → {{ P }} e @ E {{ Φ }}.
 Proof.
   intros; rewrite -{1}always_const. apply (always_intro _ _), impl_intro_l.
   by rewrite always_const right_id.
@@ -39,21 +39,21 @@ Lemma ht_val E v :
   {{ True : iProp Λ Σ }} of_val v @ E {{ λ v', v = v' }}.
 Proof. apply ht_alt. by rewrite -wp_value'; apply const_intro. Qed.
 
-Lemma ht_vs E P P' Q Q' e :
-  ((P ={E}=> P') ∧ {{ P' }} e @ E {{ Q' }} ∧ ∀ v, Q' v ={E}=> Q v)
-  ⊑ {{ P }} e @ E {{ Q }}.
+Lemma ht_vs E P P' Φ Φ' e :
+  ((P ={E}=> P') ∧ {{ P' }} e @ E {{ Φ' }} ∧ ∀ v, Φ' v ={E}=> Φ v)
+  ⊑ {{ P }} e @ E {{ Φ }}.
 Proof.
   apply (always_intro _ _), impl_intro_l.
   rewrite (assoc _ P) {1}/vs always_elim impl_elim_r.
   rewrite assoc pvs_impl_r pvs_always_r wp_always_r.
-  rewrite -(pvs_wp E e Q) -(wp_pvs E e Q); apply pvs_mono, wp_mono=> v.
+  rewrite -(pvs_wp E e Φ) -(wp_pvs E e Φ); apply pvs_mono, wp_mono=> v.
   by rewrite (forall_elim v) {1}/vs always_elim impl_elim_r.
 Qed.
 
-Lemma ht_atomic E1 E2 P P' Q Q' e :
+Lemma ht_atomic E1 E2 P P' Φ Φ' e :
   E2 ⊆ E1 → atomic e →
-  ((P ={E1,E2}=> P') ∧ {{ P' }} e @ E2 {{ Q' }} ∧ ∀ v, Q' v ={E2,E1}=> Q v)
-  ⊑ {{ P }} e @ E1 {{ Q }}.
+  ((P ={E1,E2}=> P') ∧ {{ P' }} e @ E2 {{ Φ' }} ∧ ∀ v, Φ' v ={E2,E1}=> Φ v)
+  ⊑ {{ P }} e @ E1 {{ Φ }}.
 Proof.
   intros ??; apply (always_intro _ _), impl_intro_l.
   rewrite (assoc _ P) {1}/vs always_elim impl_elim_r.
@@ -62,9 +62,9 @@ Proof.
   by rewrite (forall_elim v) {1}/vs always_elim impl_elim_r.
 Qed.
 
-Lemma ht_bind `{LanguageCtx Λ K} E P Q Q' e :
-  ({{ P }} e @ E {{ Q }} ∧ ∀ v, {{ Q v }} K (of_val v) @ E {{ Q' }})
-  ⊑ {{ P }} K e @ E {{ Q' }}.
+Lemma ht_bind `{LanguageCtx Λ K} E P Φ Φ' e :
+  ({{ P }} e @ E {{ Φ }} ∧ ∀ v, {{ Φ v }} K (of_val v) @ E {{ Φ' }})
+  ⊑ {{ P }} K e @ E {{ Φ' }}.
 Proof.
   intros; apply (always_intro _ _), impl_intro_l.
   rewrite (assoc _ P) {1}/ht always_elim impl_elim_r.
@@ -72,37 +72,36 @@ Proof.
   by rewrite (forall_elim v) /ht always_elim impl_elim_r.
 Qed.
 
-Lemma ht_mask_weaken E1 E2 P Q e :
-  E1 ⊆ E2 → {{ P }} e @ E1 {{ Q }} ⊑ {{ P }} e @ E2 {{ Q }}.
+Lemma ht_mask_weaken E1 E2 P Φ e :
+  E1 ⊆ E2 → {{ P }} e @ E1 {{ Φ }} ⊑ {{ P }} e @ E2 {{ Φ }}.
 Proof. intros. by apply always_mono, impl_mono, wp_mask_frame_mono. Qed.
 
-Lemma ht_frame_l E P Q R e :
-  {{ P }} e @ E {{ Q }} ⊑ {{ R ★ P }} e @ E {{ λ v, R ★ Q v }}.
+Lemma ht_frame_l E P Φ R e :
+  {{ P }} e @ E {{ Φ }} ⊑ {{ R ★ P }} e @ E {{ λ v, R ★ Φ v }}.
 Proof.
   apply always_intro', impl_intro_l.
   rewrite always_and_sep_r -assoc (sep_and P) always_elim impl_elim_r.
   by rewrite wp_frame_l.
 Qed.
 
-Lemma ht_frame_r E P Q R e :
-  {{ P }} e @ E {{ Q }} ⊑ {{ P ★ R }} e @ E {{ λ v, Q v ★ R }}.
+Lemma ht_frame_r E P Φ R e :
+  {{ P }} e @ E {{ Φ }} ⊑ {{ P ★ R }} e @ E {{ λ v, Φ v ★ R }}.
 Proof. setoid_rewrite (comm _ _ R); apply ht_frame_l. Qed.
 
-Lemma ht_frame_later_l E P R e Q :
+Lemma ht_frame_later_l E P R e Φ :
   to_val e = None →
-  {{ P }} e @ E {{ Q }} ⊑ {{ ▷ R ★ P }} e @ E {{ λ v, R ★ Q v }}.
+  {{ P }} e @ E {{ Φ }} ⊑ {{ ▷ R ★ P }} e @ E {{ λ v, R ★ Φ v }}.
 Proof.
   intros; apply always_intro', impl_intro_l.
   rewrite always_and_sep_r -assoc (sep_and P) always_elim impl_elim_r.
   by rewrite wp_frame_later_l //; apply wp_mono=>v; rewrite pvs_frame_l.
 Qed.
 
-Lemma ht_frame_later_r E P R e Q :
+Lemma ht_frame_later_r E P Φ R e :
   to_val e = None →
-  {{ P }} e @ E {{ Q }} ⊑ {{ P ★ ▷ R }} e @ E {{ λ v, Q v ★ R }}.
+  {{ P }} e @ E {{ Φ }} ⊑ {{ P ★ ▷ R }} e @ E {{ λ v, Φ v ★ R }}.
 Proof.
   rewrite (comm _ _ (▷ R)%I); setoid_rewrite (comm _ _ R).
   apply ht_frame_later_l.
 Qed.
-
 End hoare.
