program_logic/weakestpre.v
@@ -9,37 +9,37 @@ Local Hint Extern 10 (✓{_} _) =>
   | H : wsat _ _ _ _ |- _ => apply wsat_valid in H; last omega
   end; solve_validN.
 
-Record wp_go {Λ Σ} (E : coPset) (Q Qfork : expr Λ → nat → iRes Λ Σ → Prop)
+Record wp_go {Λ Σ} (E : coPset) (Φ Φfork : expr Λ → nat → iRes Λ Σ → Prop)
     (k : nat) (rf : iRes Λ Σ) (e1 : expr Λ) (σ1 : state Λ) := {
   wf_safe : reducible e1 σ1;
   wp_step e2 σ2 ef :
     prim_step e1 σ1 e2 σ2 ef →
     ∃ r2 r2',
       wsat k E σ2 (r2 ⋅ r2' ⋅ rf) ∧
-      Q e2 k r2 ∧
-      ∀ e', ef = Some e' → Qfork e' k r2'
+      Φ e2 k r2 ∧
+      ∀ e', ef = Some e' → Φfork e' k r2'
 }.
 CoInductive wp_pre {Λ Σ} (E : coPset)
-     (Q : val Λ → iProp Λ Σ) : expr Λ → nat → iRes Λ Σ → Prop :=
-  | wp_pre_value n r v : pvs E E (Q v) n r → wp_pre E Q (of_val v) n r
+     (Φ : val Λ → iProp Λ Σ) : expr Λ → nat → iRes Λ Σ → Prop :=
+  | wp_pre_value n r v : pvs E E (Φ v) n r → wp_pre E Φ (of_val v) n r
   | wp_pre_step n r1 e1 :
      to_val e1 = None →
      (∀ rf k Ef σ1,
        0 < k < n → E ∩ Ef = ∅ →
        wsat (S k) (E ∪ Ef) σ1 (r1 ⋅ rf) →
-       wp_go (E ∪ Ef) (wp_pre E Q)
+       wp_go (E ∪ Ef) (wp_pre E Φ)
                       (wp_pre ⊤ (λ _, True%I)) k rf e1 σ1) →
-     wp_pre E Q e1 n r1.
+     wp_pre E Φ e1 n r1.
 Program Definition wp {Λ Σ} (E : coPset) (e : expr Λ)
-  (Q : val Λ → iProp Λ Σ) : iProp Λ Σ := {| uPred_holds := wp_pre E Q e |}.
+  (Φ : val Λ → iProp Λ Σ) : iProp Λ Σ := {| uPred_holds := wp_pre E Φ e |}.
 Next Obligation.
-  intros Λ Σ E e Q r1 r2 n Hwp Hr.
+  intros Λ Σ E e Φ r1 r2 n Hwp Hr.
   destruct Hwp as [|n r1 e2 ? Hgo]; constructor; rewrite -?Hr; auto.
   intros rf k Ef σ1 ?; rewrite -(dist_le _ _ _ _ Hr); naive_solver.
 Qed.
 Next Obligation.
-  intros Λ Σ E e Q r1 r2 n1; revert Q E e r1 r2.
-  induction n1 as [n1 IH] using lt_wf_ind; intros Q E e r1 r1' n2.
+  intros Λ Σ E e Φ r1 r2 n1; revert Φ E e r1 r2.
+  induction n1 as [n1 IH] using lt_wf_ind; intros Φ E e r1 r1' n2.
   destruct 1 as [|n1 r1 e1 ? Hgo].
   - constructor; eauto using uPred_weaken.
   - intros [rf' Hr] ??; constructor; [done|intros rf k Ef σ1 ???].
@@ -54,7 +54,7 @@ Instance: Params (@wp) 4.
 Section wp.
 Context {Λ : language} {Σ : iFunctor}.
 Implicit Types P : iProp Λ Σ.
-Implicit Types Q : val Λ → iProp Λ Σ.
+Implicit Types Φ : val Λ → iProp Λ Σ.
 Implicit Types v : val Λ.
 Implicit Types e : expr Λ.
 Transparent uPred_holds.
@@ -62,10 +62,10 @@ Transparent uPred_holds.
 Global Instance wp_ne E e n :
   Proper (pointwise_relation _ (dist n) ==> dist n) (@wp Λ Σ E e).
 Proof.
-  cut (∀ Q1 Q2, (∀ v, Q1 v ≡{n}≡ Q2 v) →
-    ∀ r n', n' ≤ n → ✓{n'} r → wp E e Q1 n' r → wp E e Q2 n' r).
-  { by intros help Q Q' HQ; split; apply help. }
-  intros Q1 Q2 HQ r n'; revert e r.
+  cut (∀ Φ Ψ, (∀ v, Φ v ≡{n}≡ Ψ v) →
+    ∀ r n', n' ≤ n → ✓{n'} r → wp E e Φ n' r → wp E e Ψ n' r).
+  { by intros help Φ Ψ HΦΨ; split; apply help. }
+  intros Φ Ψ HΦΨ r n'; revert e r.
   induction n' as [n' IH] using lt_wf_ind=> e r.
   destruct 3 as [n' r v HpvsQ|n' r e1 ? Hgo].
   { constructor. by eapply pvs_ne, HpvsQ; eauto. }
@@ -78,12 +78,12 @@ Qed.
 Global Instance wp_proper E e :
   Proper (pointwise_relation _ (≡) ==> (≡)) (@wp Λ Σ E e).
 Proof.
-  by intros Q Q' ?; apply equiv_dist=>n; apply wp_ne=>v; apply equiv_dist.
+  by intros Φ Φ' ?; apply equiv_dist=>n; apply wp_ne=>v; apply equiv_dist.
 Qed.
-Lemma wp_mask_frame_mono E1 E2 e Q1 Q2 :
-  E1 ⊆ E2 → (∀ v, Q1 v ⊑ Q2 v) → wp E1 e Q1 ⊑ wp E2 e Q2.
+Lemma wp_mask_frame_mono E1 E2 e Φ Ψ :
+  E1 ⊆ E2 → (∀ v, Φ v ⊑ Ψ v) → wp E1 e Φ ⊑ wp E2 e Ψ.
 Proof.
-  intros HE HQ r n; revert e r; induction n as [n IH] using lt_wf_ind=> e r.
+  intros HE HΦ r n; revert e r; induction n as [n IH] using lt_wf_ind=> e r.
   destruct 2 as [n' r v HpvsQ|n' r e1 ? Hgo].
   { constructor; eapply pvs_mask_frame_mono, HpvsQ; eauto. }
   constructor; [done|]=> rf k Ef σ1 ???.
@@ -95,19 +95,19 @@ Proof.
   exists r2, r2'; split_ands; [rewrite HE'|eapply IH|]; eauto.
 Qed.
 
-Lemma wp_value_inv E Q v n r : wp E (of_val v) Q n r → pvs E E (Q v) n r.
+Lemma wp_value_inv E Φ v n r : wp E (of_val v) Φ n r → pvs E E (Φ v) n r.
 Proof.
   by inversion 1 as [|??? He]; [|rewrite ?to_of_val in He]; simplify_eq.
 Qed.
-Lemma wp_step_inv E Ef Q e k n σ r rf :
+Lemma wp_step_inv E Ef Φ e k n σ r rf :
   to_val e = None → 0 < k < n → E ∩ Ef = ∅ →
-  wp E e Q n r → wsat (S k) (E ∪ Ef) σ (r ⋅ rf) →
-  wp_go (E ∪ Ef) (λ e, wp E e Q) (λ e, wp ⊤ e (λ _, True%I)) k rf e σ.
+  wp E e Φ n r → wsat (S k) (E ∪ Ef) σ (r ⋅ rf) →
+  wp_go (E ∪ Ef) (λ e, wp E e Φ) (λ e, wp ⊤ e (λ _, True%I)) k rf e σ.
 Proof. intros He; destruct 3; [by rewrite ?to_of_val in He|eauto]. Qed.
 
-Lemma wp_value' E Q v : Q v ⊑ wp E (of_val v) Q.
+Lemma wp_value' E Φ v : Φ v ⊑ wp E (of_val v) Φ.
 Proof. by constructor; apply pvs_intro. Qed.
-Lemma pvs_wp E e Q : pvs E E (wp E e Q) ⊑ wp E e Q.
+Lemma pvs_wp E e Φ : pvs E E (wp E e Φ) ⊑ wp E e Φ.
 Proof.
   intros r n ? Hvs.
   destruct (to_val e) as [v|] eqn:He; [apply of_to_val in He; subst|].
@@ -117,24 +117,24 @@ Proof.
   destruct (Hvs rf (S k) Ef σ1) as (r'&Hwp&?); auto.
   eapply wp_step_inv with (S k) r'; eauto.
 Qed.
-Lemma wp_pvs E e Q : wp E e (λ v, pvs E E (Q v)) ⊑ wp E e Q.
+Lemma wp_pvs E e Φ : wp E e (λ v, pvs E E (Φ v)) ⊑ wp E e Φ.
 Proof.
-  intros r n; revert e r; induction n as [n IH] using lt_wf_ind=> e r Hr HQ.
+  intros r n; revert e r; induction n as [n IH] using lt_wf_ind=> e r Hr HΦ.
   destruct (to_val e) as [v|] eqn:He; [apply of_to_val in He; subst|].
-  { constructor; apply pvs_trans', (wp_value_inv _ (pvs E E ∘ Q)); auto. }
+  { constructor; apply pvs_trans', (wp_value_inv _ (pvs E E ∘ Φ)); auto. }
   constructor; [done|]=> rf k Ef σ1 ???.
-  destruct (wp_step_inv E Ef (pvs E E ∘ Q) e k n σ1 r rf) as [? Hstep]; auto.
+  destruct (wp_step_inv E Ef (pvs E E ∘ Φ) e k n σ1 r rf) as [? Hstep]; auto.
   split; [done|intros e2 σ2 ef ?].
   destruct (Hstep e2 σ2 ef) as (r2&r2'&?&Hwp'&?); auto.
   exists r2, r2'; split_ands; [|apply (IH k)|]; auto.
 Qed.
-Lemma wp_atomic E1 E2 e Q :
-  E2 ⊆ E1 → atomic e → pvs E1 E2 (wp E2 e (λ v, pvs E2 E1 (Q v))) ⊑ wp E1 e Q.
+Lemma wp_atomic E1 E2 e Φ :
+  E2 ⊆ E1 → atomic e → pvs E1 E2 (wp E2 e (λ v, pvs E2 E1 (Φ v))) ⊑ wp E1 e Φ.
 Proof.
   intros ? He r n ? Hvs; constructor; eauto using atomic_not_val.
   intros rf k Ef σ1 ???.
   destruct (Hvs rf (S k) Ef σ1) as (r'&Hwp&?); auto.
-  destruct (wp_step_inv E2 Ef (pvs E2 E1 ∘ Q) e k (S k) σ1 r' rf)
+  destruct (wp_step_inv E2 Ef (pvs E2 E1 ∘ Φ) e k (S k) σ1 r' rf)
     as [Hsafe Hstep]; auto using atomic_not_val.
   split; [done|]=> e2 σ2 ef ?.
   destruct (Hstep e2 σ2 ef) as (r2&r2'&?&Hwp'&?); clear Hsafe Hstep; auto.
@@ -146,7 +146,7 @@ Proof.
   - by rewrite -assoc.
   - constructor; apply pvs_intro; auto.
 Qed.
-Lemma wp_frame_r E e Q R : (wp E e Q ★ R) ⊑ wp E e (λ v, Q v ★ R).
+Lemma wp_frame_r E e Φ R : (wp E e Φ ★ R) ⊑ wp E e (λ v, Φ v ★ R).
 Proof.
   intros r' n Hvalid (r&rR&Hr&Hwp&?); revert Hvalid.
   rewrite Hr; clear Hr; revert e r Hwp.
@@ -163,8 +163,8 @@ Proof.
       (comm _ rR) !assoc -(assoc _ _ rR).
   - apply IH; eauto using uPred_weaken.
 Qed.
-Lemma wp_frame_later_r E e Q R :
-  to_val e = None → (wp E e Q ★ ▷ R) ⊑ wp E e (λ v, Q v ★ R).
+Lemma wp_frame_later_r E e Φ R :
+  to_val e = None → (wp E e Φ ★ ▷ R) ⊑ wp E e (λ v, Φ v ★ R).
 Proof.
   intros He r' n Hvalid (r&rR&Hr&Hwp&?); revert Hvalid; rewrite Hr; clear Hr.
   destruct Hwp as [|n r e ? Hgo]; [by rewrite to_of_val in He|].
@@ -178,8 +178,8 @@ Proof.
   - apply wp_frame_r; [auto|exists r2, rR; split_ands; auto].
     eapply uPred_weaken with rR n; eauto.
 Qed.
-Lemma wp_bind `{LanguageCtx Λ K} E e Q :
-  wp E e (λ v, wp E (K (of_val v)) Q) ⊑ wp E (K e) Q.
+Lemma wp_bind `{LanguageCtx Λ K} E e Φ :
+  wp E e (λ v, wp E (K (of_val v)) Φ) ⊑ wp E (K e) Φ.
 Proof.
   intros r n; revert e r; induction n as [n IH] using lt_wf_ind=> e r ?.
   destruct 1 as [|n r e ? Hgo]; [by apply pvs_wp|].
@@ -197,39 +197,39 @@ Qed.
 (** * Derived rules *)
 Opaque uPred_holds.
 Import uPred.
-Lemma wp_mono E e Q1 Q2 : (∀ v, Q1 v ⊑ Q2 v) → wp E e Q1 ⊑ wp E e Q2.
+Lemma wp_mono E e Φ Ψ : (∀ v, Φ v ⊑ Ψ v) → wp E e Φ ⊑ wp E e Ψ.
 Proof. by apply wp_mask_frame_mono. Qed.
 Global Instance wp_mono' E e :
   Proper (pointwise_relation _ (⊑) ==> (⊑)) (@wp Λ Σ E e).
-Proof. by intros Q Q' ?; apply wp_mono. Qed.
-Lemma wp_strip_pvs E e P Q : P ⊑ wp E e Q → pvs E E P ⊑ wp E e Q.
+Proof. by intros Φ Φ' ?; apply wp_mono. Qed.
+Lemma wp_strip_pvs E e P Φ : P ⊑ wp E e Φ → pvs E E P ⊑ wp E e Φ.
 Proof. move=>->. by rewrite pvs_wp. Qed.
-Lemma wp_value E Q e v : to_val e = Some v → Q v ⊑ wp E e Q.
+Lemma wp_value E Φ e v : to_val e = Some v → Φ v ⊑ wp E e Φ.
 Proof. intros; rewrite -(of_to_val e v) //; by apply wp_value'. Qed.
-Lemma wp_value_pvs E Q e v : to_val e = Some v → pvs E E (Q v) ⊑ wp E e Q.
+Lemma wp_value_pvs E Φ e v : to_val e = Some v → pvs E E (Φ v) ⊑ wp E e Φ.
 Proof. intros. rewrite -wp_pvs. rewrite -wp_value //. Qed.
-Lemma wp_frame_l E e Q R : (R ★ wp E e Q) ⊑ wp E e (λ v, R ★ Q v).
+Lemma wp_frame_l E e Φ R : (R ★ wp E e Φ) ⊑ wp E e (λ v, R ★ Φ v).
 Proof. setoid_rewrite (comm _ R); apply wp_frame_r. Qed.
-Lemma wp_frame_later_l E e Q R :
-  to_val e = None → (▷ R ★ wp E e Q) ⊑ wp E e (λ v, R ★ Q v).
+Lemma wp_frame_later_l E e Φ R :
+  to_val e = None → (▷ R ★ wp E e Φ) ⊑ wp E e (λ v, R ★ Φ v).
 Proof.
   rewrite (comm _ (▷ R)%I); setoid_rewrite (comm _ R).
   apply wp_frame_later_r.
 Qed.
-Lemma wp_always_l E e Q R `{!AlwaysStable R} :
-  (R ∧ wp E e Q) ⊑ wp E e (λ v, R ∧ Q v).
+Lemma wp_always_l E e Φ R `{!AlwaysStable R} :
+  (R ∧ wp E e Φ) ⊑ wp E e (λ v, R ∧ Φ v).
 Proof. by setoid_rewrite (always_and_sep_l _ _); rewrite wp_frame_l. Qed.
-Lemma wp_always_r E e Q R `{!AlwaysStable R} :
-  (wp E e Q ∧ R) ⊑ wp E e (λ v, Q v ∧ R).
+Lemma wp_always_r E e Φ R `{!AlwaysStable R} :
+  (wp E e Φ ∧ R) ⊑ wp E e (λ v, Φ v ∧ R).
 Proof. by setoid_rewrite (always_and_sep_r _ _); rewrite wp_frame_r. Qed.
-Lemma wp_impl_l E e Q1 Q2 : ((□ ∀ v, Q1 v → Q2 v) ∧ wp E e Q1) ⊑ wp E e Q2.
+Lemma wp_impl_l E e Φ Ψ : ((□ ∀ v, Φ v → Ψ v) ∧ wp E e Φ) ⊑ wp E e Ψ.
 Proof.
   rewrite wp_always_l; apply wp_mono=> // v.
   by rewrite always_elim (forall_elim v) impl_elim_l.
 Qed.
-Lemma wp_impl_r E e Q1 Q2 : (wp E e Q1 ∧ □ ∀ v, Q1 v → Q2 v) ⊑ wp E e Q2.
+Lemma wp_impl_r E e Φ Ψ : (wp E e Φ ∧ □ ∀ v, Φ v → Ψ v) ⊑ wp E e Ψ.
 Proof. by rewrite comm wp_impl_l. Qed.
-Lemma wp_mask_weaken E1 E2 e Q : E1 ⊆ E2 → wp E1 e Q ⊑ wp E2 e Q.
+Lemma wp_mask_weaken E1 E2 e Φ : E1 ⊆ E2 → wp E1 e Φ ⊑ wp E2 e Φ.
 Proof. auto using wp_mask_frame_mono. Qed.
 
 (** * Weakest-pre is a FSA. *)
@@ -237,6 +237,6 @@ Definition wp_fsa (e : expr Λ) : FSA Λ Σ (val Λ) := λ E, wp E e.
 Global Instance wp_fsa_prf : FrameShiftAssertion (atomic e) (wp_fsa e).
 Proof.
   rewrite /wp_fsa; split; auto using wp_mask_frame_mono, wp_atomic, wp_frame_r.
-  intros E Q. by rewrite -(pvs_wp E e Q) -(wp_pvs E e Q).
+  intros E Φ. by rewrite -(pvs_wp E e Φ) -(wp_pvs E e Φ).
 Qed.
 End wp.
