heap_lang/derived.v
@@ -12,49 +12,49 @@ Notation Skip := (Seq (Lit LitUnit) (Lit LitUnit)).
 
 Section derived.
 Context {Σ : iFunctor}.
-Implicit Types P : iProp heap_lang Σ.
-Implicit Types Q : val → iProp heap_lang Σ.
+Implicit Types P Q : iProp heap_lang Σ.
+Implicit Types Φ : val → iProp heap_lang Σ.
 
 (** Proof rules for the sugar *)
-Lemma wp_lam' E x ef e v Q :
-  to_val e = Some v → ▷ wp E (subst ef x v) Q ⊑ wp E (App (Lam x ef) e) Q.
+Lemma wp_lam' E x ef e v Φ :
+  to_val e = Some v → ▷ wp E (subst ef x v) Φ ⊑ wp E (App (Lam x ef) e) Φ.
 Proof. intros. by rewrite -wp_rec' ?subst_empty. Qed.
 
-Lemma wp_let' E x e1 e2 v Q :
-  to_val e1 = Some v → ▷ wp E (subst e2 x v) Q ⊑ wp E (Let x e1 e2) Q.
+Lemma wp_let' E x e1 e2 v Φ :
+  to_val e1 = Some v → ▷ wp E (subst e2 x v) Φ ⊑ wp E (Let x e1 e2) Φ.
 Proof. apply wp_lam'. Qed.
 
-Lemma wp_seq E e1 e2 Q : wp E e1 (λ _, ▷ wp E e2 Q) ⊑ wp E (Seq e1 e2) Q.
+Lemma wp_seq E e1 e2 Φ : wp E e1 (λ _, ▷ wp E e2 Φ) ⊑ wp E (Seq e1 e2) Φ.
 Proof.
   rewrite -(wp_bind [LetCtx "" e2]). apply wp_mono=>v.
   by rewrite -wp_let' //= ?to_of_val ?subst_empty.
 Qed.
 
-Lemma wp_skip E Q : ▷ (Q (LitV LitUnit)) ⊑ wp E Skip Q.
+Lemma wp_skip E Φ : ▷ (Φ (LitV LitUnit)) ⊑ wp E Skip Φ.
 Proof. rewrite -wp_seq -wp_value // -wp_value //. Qed.
 
-Lemma wp_le E (n1 n2 : Z) P Q :
-  (n1 ≤ n2 → P ⊑ ▷ Q (LitV $ LitBool true)) →
-  (n2 < n1 → P ⊑ ▷ Q (LitV $ LitBool false)) →
-  P ⊑ wp E (BinOp LeOp (Lit $ LitInt n1) (Lit $ LitInt n2)) Q.
+Lemma wp_le E (n1 n2 : Z) P Φ :
+  (n1 ≤ n2 → P ⊑ ▷ Φ (LitV $ LitBool true)) →
+  (n2 < n1 → P ⊑ ▷ Φ (LitV $ LitBool false)) →
+  P ⊑ wp E (BinOp LeOp (Lit $ LitInt n1) (Lit $ LitInt n2)) Φ.
 Proof.
   intros. rewrite -wp_bin_op //; [].
   destruct (bool_decide_reflect (n1 ≤ n2)); by eauto with omega.
 Qed.
 
-Lemma wp_lt E (n1 n2 : Z) P Q :
-  (n1 < n2 → P ⊑ ▷ Q (LitV $ LitBool true)) →
-  (n2 ≤ n1 → P ⊑ ▷ Q (LitV $ LitBool false)) →
-  P ⊑ wp E (BinOp LtOp (Lit $ LitInt n1) (Lit $ LitInt n2)) Q.
+Lemma wp_lt E (n1 n2 : Z) P Φ :
+  (n1 < n2 → P ⊑ ▷ Φ (LitV $ LitBool true)) →
+  (n2 ≤ n1 → P ⊑ ▷ Φ (LitV $ LitBool false)) →
+  P ⊑ wp E (BinOp LtOp (Lit $ LitInt n1) (Lit $ LitInt n2)) Φ.
 Proof.
   intros. rewrite -wp_bin_op //; [].
   destruct (bool_decide_reflect (n1 < n2)); by eauto with omega.
 Qed.
 
-Lemma wp_eq E (n1 n2 : Z) P Q :
-  (n1 = n2 → P ⊑ ▷ Q (LitV $ LitBool true)) →
-  (n1 ≠ n2 → P ⊑ ▷ Q (LitV $ LitBool false)) →
-  P ⊑ wp E (BinOp EqOp (Lit $ LitInt n1) (Lit $ LitInt n2)) Q.
+Lemma wp_eq E (n1 n2 : Z) P Φ :
+  (n1 = n2 → P ⊑ ▷ Φ (LitV $ LitBool true)) →
+  (n1 ≠ n2 → P ⊑ ▷ Φ (LitV $ LitBool false)) →
+  P ⊑ wp E (BinOp EqOp (Lit $ LitInt n1) (Lit $ LitInt n2)) Φ.
 Proof.
   intros. rewrite -wp_bin_op //; [].
   destruct (bool_decide_reflect (n1 = n2)); by eauto with omega.
