heap_lang/lifting.v
@@ -9,25 +9,25 @@ Local Hint Extern 0 (language.reducible _ _) => do_step ltac:(eauto 2).
 
 Section lifting.
 Context {Σ : iFunctor}.
-Implicit Types P : iProp heap_lang Σ.
-Implicit Types Q : val → iProp heap_lang Σ.
+Implicit Types P Q : iProp heap_lang Σ.
+Implicit Types Φ : val → iProp heap_lang Σ.
 Implicit Types K : ectx.
 Implicit Types ef : option expr.
 
 (** Bind. *)
-Lemma wp_bind {E e} K Q :
-  wp E e (λ v, wp E (fill K (of_val v)) Q) ⊑ wp E (fill K e) Q.
+Lemma wp_bind {E e} K Φ :
+  wp E e (λ v, wp E (fill K (of_val v)) Φ) ⊑ wp E (fill K e) Φ.
 Proof. apply weakestpre.wp_bind. Qed.
 
-Lemma wp_bindi {E e} Ki Q :
-  wp E e (λ v, wp E (fill_item Ki (of_val v)) Q) ⊑ wp E (fill_item Ki e) Q.
+Lemma wp_bindi {E e} Ki Φ :
+  wp E e (λ v, wp E (fill_item Ki (of_val v)) Φ) ⊑ wp E (fill_item Ki e) Φ.
 Proof. apply weakestpre.wp_bind. Qed.
 
 (** Base axioms for core primitives of the language: Stateful reductions. *)
-Lemma wp_alloc_pst E σ e v Q :
+Lemma wp_alloc_pst E σ e v Φ :
   to_val e = Some v →
-  (ownP σ ★ ▷ (∀ l, σ !! l = None ∧ ownP (<[l:=v]>σ) -★ Q (LocV l)))
-       ⊑ wp E (Alloc e) Q.
+  (ownP σ ★ ▷ (∀ l, σ !! l = None ∧ ownP (<[l:=v]>σ) -★ Φ (LocV l)))
+       ⊑ wp E (Alloc e) Φ.
 Proof.
   (* TODO RJ: This works around ssreflect bug #22. *)
   intros. set (φ v' σ' ef := ∃ l,
@@ -42,42 +42,42 @@ Proof.
   by rewrite (forall_elim l) right_id const_equiv // left_id wand_elim_r.
 Qed.
 
-Lemma wp_load_pst E σ l v Q :
+Lemma wp_load_pst E σ l v Φ :
   σ !! l = Some v →
-  (ownP σ ★ ▷ (ownP σ -★ Q v)) ⊑ wp E (Load (Loc l)) Q.
+  (ownP σ ★ ▷ (ownP σ -★ Φ v)) ⊑ wp E (Load (Loc l)) Φ.
 Proof.
   intros. rewrite -(wp_lift_atomic_det_step σ v σ None) ?right_id //;
     last by intros; inv_step; eauto using to_of_val.
 Qed.
 
-Lemma wp_store_pst E σ l e v v' Q :
+Lemma wp_store_pst E σ l e v v' Φ :
   to_val e = Some v → σ !! l = Some v' →
-  (ownP σ ★ ▷ (ownP (<[l:=v]>σ) -★ Q (LitV LitUnit))) ⊑ wp E (Store (Loc l) e) Q.
+  (ownP σ ★ ▷ (ownP (<[l:=v]>σ) -★ Φ (LitV LitUnit))) ⊑ wp E (Store (Loc l) e) Φ.
 Proof.
   intros. rewrite -(wp_lift_atomic_det_step σ (LitV LitUnit) (<[l:=v]>σ) None)
     ?right_id //; last by intros; inv_step; eauto.
 Qed.
 
-Lemma wp_cas_fail_pst E σ l e1 v1 e2 v2 v' Q :
+Lemma wp_cas_fail_pst E σ l e1 v1 e2 v2 v' Φ :
   to_val e1 = Some v1 → to_val e2 = Some v2 → σ !! l = Some v' → v' ≠ v1 →
-  (ownP σ ★ ▷ (ownP σ -★ Q (LitV $ LitBool false))) ⊑ wp E (Cas (Loc l) e1 e2) Q.
+  (ownP σ ★ ▷ (ownP σ -★ Φ (LitV $ LitBool false))) ⊑ wp E (Cas (Loc l) e1 e2) Φ.
 Proof.
   intros. rewrite -(wp_lift_atomic_det_step σ (LitV $ LitBool false) σ None)
     ?right_id //; last by intros; inv_step; eauto.
 Qed.
 
-Lemma wp_cas_suc_pst E σ l e1 v1 e2 v2 Q :
+Lemma wp_cas_suc_pst E σ l e1 v1 e2 v2 Φ :
   to_val e1 = Some v1 → to_val e2 = Some v2 → σ !! l = Some v1 →
-  (ownP σ ★ ▷ (ownP (<[l:=v2]>σ) -★ Q (LitV $ LitBool true)))
-  ⊑ wp E (Cas (Loc l) e1 e2) Q.
+  (ownP σ ★ ▷ (ownP (<[l:=v2]>σ) -★ Φ (LitV $ LitBool true)))
+  ⊑ wp E (Cas (Loc l) e1 e2) Φ.
 Proof.
   intros. rewrite -(wp_lift_atomic_det_step σ (LitV $ LitBool true) (<[l:=v2]>σ) None)
     ?right_id //; last by intros; inv_step; eauto.
 Qed.
 
 (** Base axioms for core primitives of the language: Stateless reductions *)
-Lemma wp_fork E e Q :
-  (▷ Q (LitV LitUnit) ★ ▷ wp (Σ:=Σ) ⊤ e (λ _, True)) ⊑ wp E (Fork e) Q.
+Lemma wp_fork E e Φ :
+  (▷ Φ (LitV LitUnit) ★ ▷ wp (Σ:=Σ) ⊤ e (λ _, True)) ⊑ wp E (Fork e) Φ.
 Proof.
   rewrite -(wp_lift_pure_det_step (Fork e) (Lit LitUnit) (Some e)) //=;
     last by intros; inv_step; eauto.
@@ -86,70 +86,72 @@ Qed.
 
 (* For the lemmas involving substitution, we only derive a preliminary version.
    The final version is defined in substitution.v. *)
-Lemma wp_rec' E f x e1 e2 v Q :
+Lemma wp_rec' E f x e1 e2 v Φ :
   to_val e2 = Some v →
-  ▷ wp E (subst (subst e1 f (RecV f x e1)) x v) Q ⊑ wp E (App (Rec f x e1) e2) Q.
+  ▷ wp E (subst (subst e1 f (RecV f x e1)) x v) Φ ⊑ wp E (App (Rec f x e1) e2) Φ.
 Proof.
   intros. rewrite -(wp_lift_pure_det_step (App _ _)
     (subst (subst e1 f (RecV f x e1)) x v) None) ?right_id //=;
     intros; inv_step; eauto.
 Qed.
 
-Lemma wp_un_op E op l l' Q :
+Lemma wp_un_op E op l l' Φ :
   un_op_eval op l = Some l' →
-  ▷ Q (LitV l') ⊑ wp E (UnOp op (Lit l)) Q.
+  ▷ Φ (LitV l') ⊑ wp E (UnOp op (Lit l)) Φ.
 Proof.
   intros. rewrite -(wp_lift_pure_det_step (UnOp op _) (Lit l') None)
     ?right_id -?wp_value //; intros; inv_step; eauto.
 Qed.
 
-Lemma wp_bin_op E op l1 l2 l' Q :
+Lemma wp_bin_op E op l1 l2 l' Φ :
   bin_op_eval op l1 l2 = Some l' →
-  ▷ Q (LitV l') ⊑ wp E (BinOp op (Lit l1) (Lit l2)) Q.
+  ▷ Φ (LitV l') ⊑ wp E (BinOp op (Lit l1) (Lit l2)) Φ.
 Proof.
   intros Heval. rewrite -(wp_lift_pure_det_step (BinOp op _ _) (Lit l') None)
     ?right_id -?wp_value //; intros; inv_step; eauto.
 Qed.
 
-Lemma wp_if_true E e1 e2 Q : ▷ wp E e1 Q ⊑ wp E (If (Lit $ LitBool true) e1 e2) Q.
+Lemma wp_if_true E e1 e2 Φ :
+  ▷ wp E e1 Φ ⊑ wp E (If (Lit $ LitBool true) e1 e2) Φ.
 Proof.
   rewrite -(wp_lift_pure_det_step (If _ _ _) e1 None)
     ?right_id //; intros; inv_step; eauto.
 Qed.
 
-Lemma wp_if_false E e1 e2 Q : ▷ wp E e2 Q ⊑ wp E (If (Lit $ LitBool false) e1 e2) Q.
+Lemma wp_if_false E e1 e2 Φ :
+  ▷ wp E e2 Φ ⊑ wp E (If (Lit $ LitBool false) e1 e2) Φ.
 Proof.
   rewrite -(wp_lift_pure_det_step (If _ _ _) e2 None)
     ?right_id //; intros; inv_step; eauto.
 Qed.
 
-Lemma wp_fst E e1 v1 e2 v2 Q :
+Lemma wp_fst E e1 v1 e2 v2 Φ :
   to_val e1 = Some v1 → to_val e2 = Some v2 →
-  ▷ Q v1 ⊑ wp E (Fst $ Pair e1 e2) Q.
+  ▷ Φ v1 ⊑ wp E (Fst $ Pair e1 e2) Φ.
 Proof.
   intros. rewrite -(wp_lift_pure_det_step (Fst _) e1 None)
     ?right_id -?wp_value //; intros; inv_step; eauto.
 Qed.
 
-Lemma wp_snd E e1 v1 e2 v2 Q :
+Lemma wp_snd E e1 v1 e2 v2 Φ :
   to_val e1 = Some v1 → to_val e2 = Some v2 →
-  ▷ Q v2 ⊑ wp E (Snd $ Pair e1 e2) Q.
+  ▷ Φ v2 ⊑ wp E (Snd $ Pair e1 e2) Φ.
 Proof.
   intros. rewrite -(wp_lift_pure_det_step (Snd _) e2 None)
     ?right_id -?wp_value //; intros; inv_step; eauto.
 Qed.
 
-Lemma wp_case_inl' E e0 v0 x1 e1 x2 e2 Q :
+Lemma wp_case_inl' E e0 v0 x1 e1 x2 e2 Φ :
   to_val e0 = Some v0 →
-  ▷ wp E (subst e1 x1 v0) Q ⊑ wp E (Case (InjL e0) x1 e1 x2 e2) Q.
+  ▷ wp E (subst e1 x1 v0) Φ ⊑ wp E (Case (InjL e0) x1 e1 x2 e2) Φ.
 Proof.
   intros. rewrite -(wp_lift_pure_det_step (Case _ _ _ _ _)
     (subst e1 x1 v0) None) ?right_id //; intros; inv_step; eauto.
 Qed.
 
-Lemma wp_case_inr' E e0 v0 x1 e1 x2 e2 Q :
+Lemma wp_case_inr' E e0 v0 x1 e1 x2 e2 Φ :
   to_val e0 = Some v0 →
-  ▷ wp E (subst e2 x2 v0) Q ⊑ wp E (Case (InjR e0) x1 e1 x2 e2) Q.
+  ▷ wp E (subst e2 x2 v0) Φ ⊑ wp E (Case (InjR e0) x1 e1 x2 e2) Φ.
 Proof.
   intros. rewrite -(wp_lift_pure_det_step (Case _ _ _ _ _)
     (subst e2 x2 v0) None) ?right_id //; intros; inv_step; eauto.
