program_logic/adequacy.v
@@ -10,64 +10,66 @@ Local Hint Extern 10 (✓{_} _) =>
 Section adequacy.
 Context {Λ : language} {Σ : iFunctor}.
 Implicit Types e : expr Λ.
-Implicit Types Q : val Λ → iProp Λ Σ.
+Implicit Types P Q : iProp Λ Σ.
+Implicit Types Φ : val Λ → iProp Λ Σ.
+Implicit Types Φs : list (val Λ → iProp Λ Σ).
 Implicit Types m : iGst Λ Σ.
 Transparent uPred_holds.
 
-Notation wptp n := (Forall3 (λ e Q r, uPred_holds (wp ⊤ e Q) n r)).
-Lemma wptp_le Qs es rs n n' :
-  ✓{n'} (big_op rs) → wptp n es Qs rs → n' ≤ n → wptp n' es Qs rs.
+Notation wptp n := (Forall3 (λ e Φ r, uPred_holds (wp ⊤ e Φ) n r)).
+Lemma wptp_le Φs es rs n n' :
+  ✓{n'} (big_op rs) → wptp n es Φs rs → n' ≤ n → wptp n' es Φs rs.
 Proof. induction 2; constructor; eauto using uPred_weaken. Qed.
-Lemma nsteps_wptp Qs k n tσ1 tσ2 rs1 :
+Lemma nsteps_wptp Φs k n tσ1 tσ2 rs1 :
   nsteps step k tσ1 tσ2 →
-  1 < n → wptp (k + n) (tσ1.1) Qs rs1 →
+  1 < n → wptp (k + n) (tσ1.1) Φs rs1 →
   wsat (k + n) ⊤ (tσ1.2) (big_op rs1) →
-  ∃ rs2 Qs', wptp n (tσ2.1) (Qs ++ Qs') rs2 ∧ wsat n ⊤ (tσ2.2) (big_op rs2).
+  ∃ rs2 Φs', wptp n (tσ2.1) (Φs ++ Φs') rs2 ∧ wsat n ⊤ (tσ2.2) (big_op rs2).
 Proof.
-  intros Hsteps Hn; revert Qs rs1.
+  intros Hsteps Hn; revert Φs rs1.
   induction Hsteps as [|k ?? tσ3 [e1 σ1 e2 σ2 ef t1 t2 ?? Hstep] Hsteps IH];
-    simplify_eq/=; intros Qs rs.
+    simplify_eq/=; intros Φs rs.
   { by intros; exists rs, []; rewrite right_id_L. }
-  intros (Qs1&?&rs1&?&->&->&?&
-    (Q&Qs2&r&rs2&->&->&Hwp&?)%Forall3_cons_inv_l)%Forall3_app_inv_l ?.
-  destruct (wp_step_inv ⊤ ∅ Q e1 (k + n) (S (k + n)) σ1 r
+  intros (Φs1&?&rs1&?&->&->&?&
+    (Φ&Φs2&r&rs2&->&->&Hwp&?)%Forall3_cons_inv_l)%Forall3_app_inv_l ?.
+  destruct (wp_step_inv ⊤ ∅ Φ e1 (k + n) (S (k + n)) σ1 r
     (big_op (rs1 ++ rs2))) as [_ Hwpstep]; eauto using values_stuck.
   { by rewrite right_id_L -big_op_cons Permutation_middle. }
   destruct (Hwpstep e2 σ2 ef) as (r2&r2'&Hwsat&?&?); auto; clear Hwpstep.
   revert Hwsat; rewrite big_op_app right_id_L=>Hwsat.
   destruct ef as [e'|].
-  - destruct (IH (Qs1 ++ Q :: Qs2 ++ [λ _, True%I])
-      (rs1 ++ r2 :: rs2 ++ [r2'])) as (rs'&Qs'&?&?).
+  - destruct (IH (Φs1 ++ Φ :: Φs2 ++ [λ _, True%I])
+      (rs1 ++ r2 :: rs2 ++ [r2'])) as (rs'&Φs'&?&?).
     { apply Forall3_app, Forall3_cons,
         Forall3_app, Forall3_cons, Forall3_nil; eauto using wptp_le. }
     { by rewrite -Permutation_middle /= (assoc (++))
         (comm (++)) /= assoc big_op_app. }
-    exists rs', ([λ _, True%I] ++ Qs'); split; auto.
-    by rewrite (assoc _ _ _ Qs') -(assoc _ Qs1).
-  - apply (IH (Qs1 ++ Q :: Qs2) (rs1 ++ r2 ⋅ r2' :: rs2)).
+    exists rs', ([λ _, True%I] ++ Φs'); split; auto.
+    by rewrite (assoc _ _ _ Φs') -(assoc _ Φs1).
+  - apply (IH (Φs1 ++ Φ :: Φs2) (rs1 ++ r2 ⋅ r2' :: rs2)).
     { rewrite /option_list right_id_L.
       apply Forall3_app, Forall3_cons; eauto using wptp_le.
       apply uPred_weaken with r2 (k + n); eauto using cmra_included_l. }
     by rewrite -Permutation_middle /= big_op_app.
 Qed.
-Lemma ht_adequacy_steps P Q k n e1 t2 σ1 σ2 r1 :
-  {{ P }} e1 @ ⊤ {{ Q }} →
+Lemma ht_adequacy_steps P Φ k n e1 t2 σ1 σ2 r1 :
+  {{ P }} e1 @ ⊤ {{ Φ }} →
   nsteps step k ([e1],σ1) (t2,σ2) →
   1 < n → wsat (k + n) ⊤ σ1 r1 →
   P (k + n) r1 →
-  ∃ rs2 Qs', wptp n t2 (Q :: Qs') rs2 ∧ wsat n ⊤ σ2 (big_op rs2).
+  ∃ rs2 Φs', wptp n t2 (Φ :: Φs') rs2 ∧ wsat n ⊤ σ2 (big_op rs2).
 Proof.
-  intros Hht ????; apply (nsteps_wptp [Q] k n ([e1],σ1) (t2,σ2) [r1]);
+  intros Hht ????; apply (nsteps_wptp [Φ] k n ([e1],σ1) (t2,σ2) [r1]);
     rewrite /big_op ?right_id; auto.
   constructor; last constructor.
   apply Hht with r1 (k + n); eauto using cmra_included_unit.
   eapply uPred.const_intro; eauto.
 Qed.
-Lemma ht_adequacy_own Q e1 t2 σ1 m σ2 :
+Lemma ht_adequacy_own Φ e1 t2 σ1 m σ2 :
   ✓m →
-  {{ ownP σ1 ★ ownG m }} e1 @ ⊤ {{ Q }} →
+  {{ ownP σ1 ★ ownG m }} e1 @ ⊤ {{ Φ }} →
   rtc step ([e1],σ1) (t2,σ2) →
-  ∃ rs2 Qs', wptp 2 t2 (Q :: Qs') rs2 ∧ wsat 2 ⊤ σ2 (big_op rs2).
+  ∃ rs2 Φs', wptp 2 t2 (Φ :: Φs') rs2 ∧ wsat 2 ⊤ σ2 (big_op rs2).
 Proof.
   intros Hv ? [k ?]%rtc_nsteps.
   eapply ht_adequacy_steps with (r1 := (Res ∅ (Excl σ1) (Some m))); eauto; [|].
@@ -91,30 +93,30 @@ Proof.
   apply wp_value_inv in Hwp; destruct (Hwp (big_op rs) 2 ∅ σ2) as [r' []]; auto.
   by rewrite right_id_L.
 Qed.
-Lemma ht_adequacy_reducible E Q e1 e2 t2 σ1 m σ2 :
+Lemma ht_adequacy_reducible E Φ e1 e2 t2 σ1 m σ2 :
   ✓ m →
-  {{ ownP σ1 ★ ownG m }} e1 @ E {{ Q }} →
+  {{ ownP σ1 ★ ownG m }} e1 @ E {{ Φ }} →
   rtc step ([e1], σ1) (t2, σ2) →
   e2 ∈ t2 → to_val e2 = None → reducible e2 σ2.
 Proof.
   intros Hv ? Hs [i ?]%elem_of_list_lookup He.
-  destruct (ht_adequacy_own Q e1 t2 σ1 m σ2) as (rs2&Qs&?&?); auto.
+  destruct (ht_adequacy_own Φ e1 t2 σ1 m σ2) as (rs2&Φs&?&?); auto.
   { by rewrite -(ht_mask_weaken E ⊤). }
-  destruct (Forall3_lookup_l (λ e Q r, wp ⊤ e Q 2 r) t2
-    (Q :: Qs) rs2 i e2) as (Q'&r2&?&?&Hwp); auto.
-  destruct (wp_step_inv ⊤ ∅ Q' e2 1 2 σ2 r2 (big_op (delete i rs2)));
+  destruct (Forall3_lookup_l (λ e Φ r, wp ⊤ e Φ 2 r) t2
+    (Φ :: Φs) rs2 i e2) as (Φ'&r2&?&?&Hwp); auto.
+  destruct (wp_step_inv ⊤ ∅ Φ' e2 1 2 σ2 r2 (big_op (delete i rs2)));
     rewrite ?right_id_L ?big_op_delete; auto.
 Qed.
-Theorem ht_adequacy_safe E Q e1 t2 σ1 m σ2 :
+Theorem ht_adequacy_safe E Φ e1 t2 σ1 m σ2 :
   ✓ m →
-  {{ ownP σ1 ★ ownG m }} e1 @ E {{ Q }} →
+  {{ ownP σ1 ★ ownG m }} e1 @ E {{ Φ }} →
   rtc step ([e1], σ1) (t2, σ2) →
   Forall (λ e, is_Some (to_val e)) t2 ∨ ∃ t3 σ3, step (t2, σ2) (t3, σ3).
 Proof.
   intros.
   destruct (decide (Forall (λ e, is_Some (to_val e)) t2)) as [|Ht2]; [by left|].
   apply (not_Forall_Exists _), Exists_exists in Ht2; destruct Ht2 as (e2&?&He2).
-  destruct (ht_adequacy_reducible E Q e1 e2 t2 σ1 m σ2) as (e3&σ3&ef&?);
+  destruct (ht_adequacy_reducible E Φ e1 e2 t2 σ1 m σ2) as (e3&σ3&ef&?);
     rewrite ?eq_None_not_Some; auto.
   destruct (elem_of_list_split t2 e2) as (t2'&t2''&->); auto.
   right; exists (t2' ++ e3 :: t2'' ++ option_list ef), σ3; econstructor; eauto.
