program_logic/lifting.v
@@ -12,19 +12,20 @@ Context {Λ : language} {Σ : iFunctor}.
 Implicit Types v : val Λ.
 Implicit Types e : expr Λ.
 Implicit Types σ : state Λ.
-Implicit Types Q : val Λ → iProp Λ Σ.
+Implicit Types P Q : iProp Λ Σ.
+Implicit Types Φ : val Λ → iProp Λ Σ.
 Transparent uPred_holds.
 
 Notation wp_fork ef := (default True ef (flip (wp ⊤) (λ _, True)))%I.
 
 Lemma wp_lift_step E1 E2
-    (φ : expr Λ → state Λ → option (expr Λ) → Prop) Q e1 σ1 :
+    (φ : expr Λ → state Λ → option (expr Λ) → Prop) Φ e1 σ1 :
   E1 ⊆ E2 → to_val e1 = None →
   reducible e1 σ1 →
   (∀ e2 σ2 ef, prim_step e1 σ1 e2 σ2 ef → φ e2 σ2 ef) →
   pvs E2 E1 (ownP σ1 ★ ▷ ∀ e2 σ2 ef,
-    (■ φ e2 σ2 ef ∧ ownP σ2) -★ pvs E1 E2 (wp E2 e2 Q ★ wp_fork ef))
-  ⊑ wp E2 e1 Q.
+    (■ φ e2 σ2 ef ∧ ownP σ2) -★ pvs E1 E2 (wp E2 e2 Φ ★ wp_fork ef))
+  ⊑ wp E2 e1 Φ.
 Proof.
   intros ? He Hsafe Hstep r n ? Hvs; constructor; auto.
   intros rf k Ef σ1' ???; destruct (Hvs rf (S k) Ef σ1')
@@ -40,11 +41,11 @@ Proof.
   by exists r1', r2'; split_ands; [| |by intros ? ->].
 Qed.
 
-Lemma wp_lift_pure_step E (φ : expr Λ → option (expr Λ) → Prop) Q e1 :
+Lemma wp_lift_pure_step E (φ : expr Λ → option (expr Λ) → Prop) Φ e1 :
   to_val e1 = None →
   (∀ σ1, reducible e1 σ1) →
   (∀ σ1 e2 σ2 ef, prim_step e1 σ1 e2 σ2 ef → σ1 = σ2 ∧ φ e2 ef) →
-  (▷ ∀ e2 ef, ■ φ e2 ef → wp E e2 Q ★ wp_fork ef) ⊑ wp E e1 Q.
+  (▷ ∀ e2 ef, ■ φ e2 ef → wp E e2 Φ ★ wp_fork ef) ⊑ wp E e1 Φ.
 Proof.
   intros He Hsafe Hstep r n ? Hwp; constructor; auto.
   intros rf k Ef σ1 ???; split; [done|]. destruct n as [|n]; first lia.
@@ -57,14 +58,14 @@ Qed.
 Opaque uPred_holds.
 Import uPred.
 
-Lemma wp_lift_atomic_step {E Q} e1
+Lemma wp_lift_atomic_step {E Φ} e1
     (φ : val Λ → state Λ → option (expr Λ) → Prop) σ1 :
   to_val e1 = None →
   reducible e1 σ1 →
   (∀ e2 σ2 ef,
     prim_step e1 σ1 e2 σ2 ef → ∃ v2, to_val e2 = Some v2 ∧ φ v2 σ2 ef) →
-  (ownP σ1 ★ ▷ ∀ v2 σ2 ef, ■ φ v2 σ2 ef ∧ ownP σ2 -★ Q v2 ★ wp_fork ef)
-  ⊑ wp E e1 Q.
+  (ownP σ1 ★ ▷ ∀ v2 σ2 ef, ■ φ v2 σ2 ef ∧ ownP σ2 -★ Φ v2 ★ wp_fork ef)
+  ⊑ wp E e1 Φ.
 Proof.
   intros. rewrite -(wp_lift_step E E (λ e2 σ2 ef, ∃ v2,
     to_val e2 = Some v2 ∧ φ v2 σ2 ef) _ e1 σ1) //; [].
@@ -78,12 +79,12 @@ Proof.
   by rewrite left_id wand_elim_r -(wp_value _ _ e2' v2').
 Qed.
 
-Lemma wp_lift_atomic_det_step {E Q e1} σ1 v2 σ2 ef :
+Lemma wp_lift_atomic_det_step {E Φ e1} σ1 v2 σ2 ef :
   to_val e1 = None →
   reducible e1 σ1 →
   (∀ e2' σ2' ef', prim_step e1 σ1 e2' σ2' ef' →
     σ2 = σ2' ∧ to_val e2' = Some v2 ∧ ef = ef') →
-  (ownP σ1 ★ ▷ (ownP σ2 -★ Q v2 ★ wp_fork ef)) ⊑ wp E e1 Q.
+  (ownP σ1 ★ ▷ (ownP σ2 -★ Φ v2 ★ wp_fork ef)) ⊑ wp E e1 Φ.
 Proof.
   intros. rewrite -(wp_lift_atomic_step _ (λ v2' σ2' ef',
     σ2 = σ2' ∧ v2 = v2' ∧ ef = ef') σ1) //; last naive_solver.
@@ -94,11 +95,11 @@ Proof.
   apply const_elim_l=>-[-> [-> ->]] /=. by rewrite wand_elim_r.
 Qed.
 
-Lemma wp_lift_pure_det_step {E Q} e1 e2 ef :
+Lemma wp_lift_pure_det_step {E Φ} e1 e2 ef :
   to_val e1 = None →
   (∀ σ1, reducible e1 σ1) →
   (∀ σ1 e2' σ2 ef', prim_step e1 σ1 e2' σ2 ef' → σ1 = σ2 ∧ e2 = e2' ∧ ef = ef')→
-  ▷ (wp E e2 Q ★ wp_fork ef) ⊑ wp E e1 Q.
+  ▷ (wp E e2 Φ ★ wp_fork ef) ⊑ wp E e1 Φ.
 Proof.
   intros.
   rewrite -(wp_lift_pure_step E (λ e2' ef', e2 = e2' ∧ ef = ef') _ e1) //=.
